working parser need to prove termination

jsonParserScript.sml
@@ -5,8 +5,13 @@
 4. Put recursion where possible
 5. add comprehensive tests
 6. Termination proofs
-7. Write descriptimn in the begining
+7. Write description in the begining
+8. Error message: make it uniform i.e return index and the only one character
+9. fix Number parser error message:
+jsonNumber_parser.run (Input 0 "--123456789") =
+Failure (ParserError 1 "Expected digits, but found '1'"): thm
  *)
+ 
 
 
 
@@ -14,15 +19,27 @@
 open stringTheory; (* string *)
 open listTheory; (* LENGTH_CONS TAKE*)
 open extra_stringTheory; (* EXTRACT *)
+open arithmeticTheory;  (* SUC_ONE_ADD EXP*)
+open mlstringTheory; (* int *)
+open jsonLangTheory; (* obj *)
+(*
+FOR REFERENCE:
+val _ = Datatype`
+  obj =
+     Object ((mlstring # obj ) list)
+   | Array (obj list)
+   | String mlstring
+   | Int int
+   | Bool bool
+   | Null`;
 
-(* Drafting *)     
-open jsonLangTheory;
-open mlstringTheory;
+*)  
+
 
 (*
-Not imported 
+Not imported
+open jsonLangTheory;
 open PSLPathTheory; (* CONS_def *)
-open arithmeticTheory; (* SUC_ONE_ADD *)
 open sexpcodeTheory; (* STRING_def*)
 open source_valuesTheory; (* option_def *)
 open optionTheory; (* SOME THE NONE*)
@@ -78,6 +95,47 @@ End
 Theorem cons_lenght_thm:
   ∀s x xs. (LENGTH s > 0) ⇒ LENGTH (TL s) < LENGTH s
 Proof
+  wf_rel_tac `measure (\s. LENGTH s)`  (* The well-founded measure is the length of the list *)
+  THEN REWRITE_TAC [LENGTH_TL]         (* Rewrite using the definition of TL *)
+  THEN INDUCT_TAC                      (* Apply induction over the structure of the list *)
+  THEN ASM_REWRITE_TAC []              (* Simplify using the assumptions *)
+  THEN ARITH_TAC                       (* Use arithmetic tactics to complete the proof *)
+QED
+
+
+
+        
+
+
+Theorem cons_lenght_thm:
+  ∀s x xs. (LENGTH s > 0) ⇒ LENGTH (TL s) < LENGTH s
+
+Proof
+  (* Start by applying induction on the structure of the list `s` *)
+  Induct_on ‘s’>>
+
+  (* Case 1: `s` is the empty list, but LENGTH s > 0 eliminates this case *)
+  (* Thus, we automatically move to the second case *)
+
+  (* Case 2: `s = x::xs` *)
+  STRIP_TAC>>
+
+  (* Now, we need to prove LENGTH(TL (x::xs)) < LENGTH(x::xs). Simplify this expression *)
+  REWRITE_TAC [TL]>>
+
+  (* TL (x::xs) = xs, so we need to show LENGTH(xs) < LENGTH(x::xs) *)
+  REWRITE_TAC [LENGTH]>>
+
+  (* This reduces to proving that SUC (LENGTH xs) > LENGTH xs *)
+  ARITH_TAC
+
+QED
+
+        
+
+Theorem cons_lenght_thm:
+  ∀s x xs. (LENGTH s > 0) ⇒ LENGTH (TL s) < LENGTH s
+Proof
   fs[LENGTH_TL]
 QED
  
@@ -106,27 +164,7 @@ Proof
   spose_not_then assume_tac >>
   fs[]   
 QED
-        
-   
-Datatype:
-  JsonValue = JsonNull
-             | JsonBool bool
-             | JsonNumber num
-             | JsonString string
-             | JsonArray (JsonValue list)
-             | JsonObject ((string # JsonValue) list)
-End
-
-
-Datatype:
-  JsonValue = JsonNull
-             | JsonBool bool
-             | JsonNumber int
-             | JsonString string
-             | JsonArray (JsonValue list)
-             | JsonObject ((string # JsonValue) list)
-End
-
+            
 
 Definition char_parser_def:
   char_parser x =
@@ -138,12 +176,13 @@ Definition char_parser_def:
                 if (FST (THE r)) = x then
                   Success ((SND (THE r)), x)
                 else
-                  Failure (ParserError (input.Location) "E")
+                  Failure (ParserError (input.Location) ("Expected '" ++ [x] ++ "', but found '" ++ input.String ++ "'"))
                 )
               else
-                Failure (ParserError (input.Location) "E")
+                Failure (ParserError (input.Location) ("Expected SOME but found NONE"))
          )
 End
+
 
 
 Theorem char_parser_success_thm:
@@ -203,8 +242,8 @@ Definition const_parser_def:
 End
 
         
-Overload "<$>"[local] = “const_parser”;
-val _ = set_fixity "<$>" (Infixl 550);
+Overload "<x>" = “const_parser”;
+val _ = set_fixity "<x>" (Infixl 550);
 
 
 Theorem const_parser_length_thm:
@@ -225,10 +264,9 @@ Proof
   ]
 QED
    
-
-(* Parser optional whitespase *)
+(*  Parser optional whitespase *)
 Definition whitespace_parser_def:
-  whitespace_parser = const_parser "" (char_parser #" ")
+  whitespace_parser = "" <x> (char_parser #" ")
 End
 
 Theorem whitespace_parser_length_thm:
@@ -250,6 +288,8 @@ Proof
   ]
 QED
 
+       
+       
         
 Definition whitespace_loop_helper_def:
   whitespace_loop_helper input =
@@ -277,25 +317,75 @@ End
 
 Overload "<|>"[local] = “alt_parser”;
 val _ = set_fixity "<|>" (Infixl 570);
-       
 
+
+Theorem alt_parser_length_thm:
+  ∀ input input' p1 p2 parsed. (alt_parser p1 p2).run input = Success(input', parsed) ⇒ STRLEN(input'.String) < STRLEN(input.String)
+Proof
+  cheat
+QED
+       
+    
+
+
+    
+
+(* parser_1 <&> parser_2 
+Definition parser_sequenser_string_def:
+  parser_sequenser_string p2 p1 =
+  Parser (λ input1.
+            case p1.run input1 of
+              Success (input2, parsed1) =>
+                (
+                case p2.run input2 of
+                  Success (input3, parsed2) =>
+                    let
+                      parsed = "" ++ parsed1 ++ parsed2
+                    in
+                        Success (input3, parsed)
+                | Failure err => Failure err
+                )
+            | Failure err => Failure err
+         )
+End
+ *)
+
+(* New version *) 
+Definition parser_sequenser_string_def:
+  parser_sequenser_string p2 p1 =
+  Parser (λ input1.
+            case p1.run input1 of
+              Success (input2, parsed1) =>
+                (
+                case p2.run input2 of
+                  Success (input3, parsed2) =>
+                    let
+                      parsed = [] ++ parsed1 ++ parsed2
+                    in
+                        Success (input3, parsed)
+                | Failure err => Failure err
+                )
+            | Failure err => Failure err
+         )
+End
+
+        
+
+(* Overloading for short-hand notation *)
+Overload "<&>"[local] = “parser_sequenser_string”;
+val _ = set_fixity "<&>" (Infixl 520);
+
+(* Joiner: Output -> Output*)
 Definition string_parser_joiner_def:
   string_parser_joiner p = λ output.
                              case output of
-                               (* if the input is good then apply parser *)
                                Success (input1, parsed1) =>
-                                 (
-                                 case p.run(input1) of
-                                   (* if parsed succeeds then attach the input to the result and return *)
+                                 ( case p.run(input1) of
                                    Success (input2, parsed2)  => Success (input2, (parsed1 ++ [parsed2]))
-                                 (* if parser fails the return the original input *)
                                  |  Failure err => output)
-                             (* if input is bad then return it as it is*)
                              | Failure err => Failure err
 End
 
-
-        
 
 Definition SWAP_ARGS_def:
   SWAP_ARGS f = λx y. f y x
@@ -321,18 +411,18 @@ Definition true_parser_def:
   Parser (λ input.
             if LENGTH input.String >= 4 then
               case (string_parser "true").run (Input input.Location (TAKE 4 input.String))  of 
-                Success (input'', "true") => Success ((Input input''.Location (DROP 4 input.String)), JsonBool T)
+                Success (input'', "true") => Success ((Input input''.Location (DROP 4 input.String)), Bool T)
               | Failure e => Failure e
             else Failure (ParserError input.Location "Expected string of length grater than 3 but found shorter")
          )                          
-End
+End     
 
 Definition false_parser_def:
   false_parser =
   Parser (λ input.
             if LENGTH input.String >= 5 then
               case (string_parser "false").run (Input input.Location (TAKE 5 input.String))  of 
-                Success (input'', "false") => Success ((Input input''.Location (DROP 5 input.String)), JsonBool F)
+                Success (input'', "false") => Success ((Input input''.Location (DROP 5 input.String)), Bool F)
               | Failure e => Failure e
             else Failure (ParserError input.Location "Expected string of length grater than 4 but found shorter")
          )                          
@@ -349,20 +439,13 @@ Definition jsonNull_parser_def:
   Parser (λ input.
             if LENGTH input.String >= 4 then
               case (string_parser "null").run (Input input.Location (TAKE 4 input.String))  of 
-                Success (input'', "null") => Success ((Input input''.Location (DROP 4 input.String)), JsonNull)
+                Success (input'', "null") => Success ((Input input''.Location (DROP 4 input.String)), Null)
               | Failure e => Failure e
             else Failure (ParserError input.Location "Expected string of length grater than 3 but found shorter")
          )                          
 End
 
 
-Definition first_is_minus_def:
-  first_is_minus s = case s of
-                       "" => F
-                     | _ => SUBSTRING (s, 0, 1) = "-"     
-End
-
-        
 Definition first_is_digit_def:
   first_is_digit s = case s of
                        "" => F
@@ -374,134 +457,257 @@ Definition extract_first_digits_def:
                            else ""
 End
 
-EVAL“extract_first_digits "123 000"”;
-EVAL“(char_parser #"0").run  (Input 0 "0") ”;
-type_of“char_parser”;
 
-Definition zero_parser_def:
-  zero_parser = const_parser "" (char_parser #"-")
+Definition dec_digit_parser_def:
+  dec_digit_parser = (
+((0:int) <x> (char_parser #"0")) <|>
+((1:int) <x> (char_parser #"1")) <|>
+((2:int) <x> (char_parser #"2")) <|>
+((3:int) <x> (char_parser #"3")) <|>
+((4:int) <x> (char_parser #"4")) <|>
+((5:int) <x> (char_parser #"5")) <|>
+((6:int) <x> (char_parser #"6")) <|>
+((7:int) <x> (char_parser #"7")) <|>
+((8:int) <x> (char_parser #"8")) <|>
+((9:int) <x> (char_parser #"9"))
+)
 End
 
-Definition zero_parser_def:
-  zero_parser = const_parser 0:int (char_parser #"0")
+Definition hex_digit_helper_def:
+  hex_digit_helper = (
+((10:int) <x> (char_parser #"a")) <|>
+((10:int) <x> (char_parser #"A")) <|>
+((11:int) <x> (char_parser #"b")) <|>
+((11:int) <x> (char_parser #"B")) <|>
+((12:int) <x> (char_parser #"c")) <|>
+((12:int) <x> (char_parser #"C")) <|>
+((13:int) <x> (char_parser #"d")) <|>
+((13:int) <x> (char_parser #"D")) <|>
+((14:int) <x> (char_parser #"e")) <|>
+((14:int) <x> (char_parser #"E")) <|>
+((15:int) <x> (char_parser #"f")) <|>
+((15:int) <x> (char_parser #"F")) 
+)
 End
 
-        
-Definition character_parser_def:
-  character_parser c v = (λ x. if c = x then SOME v else NONE)                                              
+Definition hex_digit_parser_def:
+  hex_digit_parser = (dec_digit_parser <|> hex_digit_helper)
+End
+                            
+Definition extract_def:
+  extract r = case r of
+                Success (input, parsed) => SOME parsed
+              |_ => NONE
 End
 
-(* for p in parsers 
-       if *)        
-
-type_of“(character_parser #"0" (0:int))”
-EVAL“(character_parser #"0" (0:int)) #"0"”;  
-        
-(*returns v if p was successul *)
-Definition const_parser_def:
-  const_parser v p =
-  Parser (λ input.
-      case p.run input of
-        Success (rest, _) => Success (rest, v)
-      | Failure err => Failure err)
-End        
-        
+     
+(* Assuming the input string contains only digits and the parsed component is 0 to start with*)
+Definition dec_digit_parser_joiner_def[tailrecursive]:
+  dec_digit_parser_joiner output
+  = case output of
+      Success (input0, parsed0) =>
+        (case (dec_digit_parser.run input0) of
+          Success (input1, parsed1) => dec_digit_parser_joiner (Success (input1, (parsed0 + (10 ** ((LENGTH input0.String)-1)) * parsed1)))
+        | Failure err => output)
+    | Failure err => Failure err
+End
 
 Definition minus_parser_def:
-  minus_parser = const_parser "" (char_parser #"-")
+  minus_parser = "" <x> (char_parser #"-")
 End
 
-(* assume the input is a string of digints with optional leading minus *)
-Definition toInt_def:
-  toInt s = if (first_is_minus s) then 0-t
+Definition dec_str_to_int_def:
+  dec_str_to_int s = THE(extract(dec_digit_parser_joiner (Success ((Input 0 s), (0:int)))))
 End
 
-Definition toInt_def:
-  toInt s = if (first_is_minus s) then 0-t
-EndDefinition
-
-        
-EVAL“LENGTH "1234"”;
-EVAL“SUBSTRING ("1234", 0, 4)”  ;
-EVAL“ -1:int * (toNum "4"):int ”;
-
-
-toNum parsed_digits_string
-        
-
-type_of“minus_parser.run”;
-EVAL “minus_parser.run (Input 0 "-123")”;
-type_of“minus_parser.run”;
-EVAL“first_is_digit "1"”;
-
-EVAL“(0-2):int”;
-type_of“(0-2):int”;
-type_of“(3:num):int”;
-
-
-Definition integer_parser_precursor_def:
-  integer_parser_precursor input = if first_is_digit input.String then
-                                     (
-                                        
-
-
-                                      case minus_parser.run input of
-                                        
-End  
+Definition dec_str_to_negative_int_def:
+  dec_str_to_negative_int s = 0 - THE(extract(dec_digit_parser_joiner (Success ((Input 0 s), (0:int)))))
+End        
 
 
 (* TODO redo using recursion *)
-Definition jsonNumber_parser_def:
-  jsonNumber_parser = Parser (λ input.
-                                case input of
-                                  Input location "" => Failure (ParserError location ("Expected digits, but reached end of string"))
-                                | Input location1 string1 =>
-                                    let parsed_digits_list = extract_first_digits string1
-                                    in
-                                      case parsed_digits_list of
-                                        "" =>
-                                          let first_character_string = SUBSTRING (input.String, input.Location, 1)
-                                          in
-                                            Failure (ParserError location1 ("Expected digits, but found '" ++ first_character_string ++ "'"))
-                                            | parsed_digits_string =>
-                                                let string2 = EXTRACT (string1, (LENGTH parsed_digits_list), NONE)
-                                                in
-                                                  Success (Input (location1 + LENGTH parsed_digits_string) string2,  (JsonNumber (toNum parsed_digits_string)))
-                                                  | _ => Failure (ParserError location ("Expected digits, but found '" ++ input.String ++ "'"))
+Definition jsonNumber_dec_non_negative_parser_def:
+  jsonNumber_dec_non_negative_parser =
+  Parser (λ input.
+            case input of
+
+              (*if nothing to parse*)
+              Input location "" => Failure (ParserError location ("Expected digits, but reached end of string"))
+
+            (* if something to parse *)                           
+            | Input location1 string1 =>
+
+                (* get first digits *)
+                let parsed_digits_list = extract_first_digits string1
+                in
+
+                  (* chek if there are digits *)
+                  case parsed_digits_list of
+
+                    (* if no digits then Fail *)
+                    "" =>
+
+                      let first_character_string = SUBSTRING (input.String, input.Location, 1)
+                      in
+                        Failure (ParserError location1 ("Expected digits, but found '" ++ first_character_string ++ "'"))
+
+                        (* if thre are some digits *)                     
+                        | parsed_digits_string =>
+
+                            (* extract the substring containing only digits*)
+                            let string2 = EXTRACT (string1, (LENGTH parsed_digits_list), NONE)
+                            in
+
+                              (* convert digiut string to Num and return *)
+                              Success (Input (location1 + LENGTH parsed_digits_string) string2,  (Int (dec_str_to_int parsed_digits_string)))
+                              | _ => Failure (ParserError location ("Expected digits, but found '" ++ input.String ++ "'"))
+         )
+End
+
+Definition jsonNumber_dec_negative_parser_def:
+  jsonNumber_dec_negative_parser =
+  Parser (λ input.
+            case input of
+
+              (*if nothing to parse*)
+              Input location "" => Failure (ParserError location ("Expected digits, but reached end of string"))
+
+            (* if something to parse *)                           
+            | Input location1 string1 =>
+
+                (* get first digits *)
+                let parsed_digits_list = extract_first_digits string1
+                in
+
+                  (* chek if there are digits *)
+                  case parsed_digits_list of
+
+                    (* if no digits then Fail *)
+                    "" =>
+
+                      let first_character_string = SUBSTRING (input.String, input.Location, 1)
+                      in
+                        Failure (ParserError location1 ("Expected digits, but found '" ++ first_character_string ++ "'"))
+
+                        (* if thre are some digits *)                     
+                        | parsed_digits_string =>
+
+                            (* extract the substring containing only digits*)
+                            let string2 = EXTRACT (string1, (LENGTH parsed_digits_list), NONE)
+                            in
+
+                              (* convert digiut string to Num and return *)
+                              Success (Input (location1 + LENGTH parsed_digits_string) string2,  (Int (dec_str_to_negative_int parsed_digits_string)))
+                              | _ => Failure (ParserError location ("Expected digits, but found '" ++ input.String ++ "'"))
+         )
+End
+
+          
+(* TODO: include negative numbers *)
+Definition jsonNumber_dec_parser_def:
+  jsonNumber_dec_parser = Parser (λ input.case input of
+                                        Input location "" => Failure (ParserError location ("Expected digits, but reached end of string"))                        
+                                      | Input _ _ =>
+                                          case minus_parser.run input of
+                                            Failure f => jsonNumber_dec_non_negative_parser.run input
+                                          | Success (input1, _ ) => jsonNumber_dec_negative_parser.run input1                                                                         
                              )
 End
 
-
-EVAL“jsonNumber_parser.run (Input 0 "123Something-Else")”;
-
-
-
         
-        
-Definition parser_sequenser_string_def:
-  parser_sequenser_string p2 p1 =
-  Parser (λ input1.
-            case p1.run input1 of
-              Success (input2, parsed1) =>
-                (
-                case p2.run input2 of
-                  Success (input3, parsed2) =>
-                    let
-                      parsed = "" ++ parsed1 ++ parsed2
-                    in
-                        Success (input3, parsed)
-                | Failure err => Failure err
-                )
-            | Failure err => Failure err
+Definition hex_prefix_parser_def:
+  hex_prefix_parser = ((("" <x> (char_parser #"x")) <|>
+  (const_parser "" (char_parser #"X"))) <&> ("" <x> (char_parser #"0")))
+End
+
+
+Definition hex_digit_parser_joiner_def[tailrecursive]:
+  hex_digit_parser_joiner output =
+  case output of
+    Success (input0, parsed0) =>
+      (case (hex_digit_parser.run input0) of
+        Success (input1, parsed1) =>
+          hex_digit_parser_joiner (Success (input1, (parsed0 + (16 ** ((LENGTH input0.String)-1)) * parsed1)))
+      | Failure err => output)
+  | Failure err => Failure err
+End
+
+
+Definition hex_str_to_int_def:
+  hex_str_to_int s = 0 - THE(extract(hex_digit_parser_joiner (Success ((Input 0 s), (0:int)))))
+End        
+
+
+Definition jsonNumber_hex_parser_def:
+  jsonNumber_hex_parser =
+  Parser (λ input.
+            case input of
+
+              (*if nothing to parse*)
+              Input location "" => Failure (ParserError location ("Expected digits, but reached end of string"))
+
+            (* if something to parse *)                           
+            | Input location1 string1 =>
+
+                (* get first digits *)
+                let parsed_digits_list = extract_first_digits string1
+                in
+
+                  (* chek if there are digits *)
+                  case parsed_digits_list of
+
+                    (* if no digits then Fail *)
+                    "" =>
+
+                      let first_character_string = SUBSTRING (input.String, input.Location, 1)
+                      in
+                        Failure (ParserError location1 ("Expected digits, but found '" ++ first_character_string ++ "'"))
+
+                        (* if thre are some digits *)                     
+                        | parsed_digits_string =>
+
+                            (* extract the substring containing only digits*)
+                            let string2 = EXTRACT (string1, (LENGTH parsed_digits_list), NONE)
+                            in
+
+                              (* convert digiut string to Num and return *)
+                              Success (Input (location1 + LENGTH parsed_digits_string) string2,  (Int (hex_str_to_int parsed_digits_string)))
+                              | _ => Failure (ParserError location ("Expected hex digits, but found '" ++ input.String ++ "'"))
          )
 End
-(* Overloading for short-hand notation *)
-Overload "<&>"[local] = “parser_sequenser_string”;
-val _ = set_fixity "<&>" (Infixl 520);
 
+
+
+Definition jsonNumber_parser_def:
+  jsonNumber_parser =
+  Parser (λ input.case input of
+                    Input location "" => Failure (ParserError location ("Expected digits, but reached end of string"))                        
+                  | Input _ _ =>
+                      case minus_parser.run input of
+                        Success (input1, _ ) => jsonNumber_dec_negative_parser.run input1  
+                      | Failure _ =>
+                          (case hex_prefix_parser.run input of
+                             Success (input1, _ ) => jsonNumber_hex_parser.run input1  
+                           | Failure _ => jsonNumber_dec_non_negative_parser.run input
+                          )
+         )
+End
+      
+(* PASS *)
+EVAL“jsonNumber_parser.run (Input 0 "123456789")”;             
+EVAL“jsonNumber_parser.run (Input 0 "-123456789")”;
+EVAL“jsonNumber_parser.run (Input 0 "0x123456789")”;
+EVAL“jsonNumber_parser.run (Input 0 "1x23456789")”;
+EVAL“jsonNumber_parser.run (Input 0 "0x0123456789")”;
+EVAL“jsonNumber_parser.run (Input 0 "-0")”;
+
+(* FAIL *)
+EVAL“jsonNumber_parser.run (Input 0 "-0x123456789")”;
+EVAL“jsonNumber_parser.run (Input 0 "--123456789")”;
+EVAL“jsonNumber_parser.run (Input 0 "+123456789")”;
 
 Definition special_char_parser_def:
-  special_char_parser = const_parser "" (char_parser (CHR 34))
+  special_char_parser = "" <x> (char_parser (CHR 34))
 End
 
 
@@ -535,147 +741,448 @@ End
 
 
 Definition stringliteral_parser_def:
-  stringliteral_parser = Parser (λ input.
-                                case (special_char_parser <&> (normal_string_parser <&> special_char_parser)).run input of
-                                  Success (input', parsed_string) =>  Success (input', parsed_string)
-                                | Failure err => Failure err
-                             )
+  stringliteral_parser =
+  Parser (λ input.
+            case (special_char_parser <&> (normal_string_parser <&> special_char_parser)).run input of
+              Success (input', parsed_string) =>  Success (input', parsed_string)
+            | Failure err => Failure err
+         )
 End
 
-
+        
 Definition jsonString_parser_def:
-  jsonString_parser = Parser (λ input.
-                                case (special_char_parser <&> (normal_string_parser <&> special_char_parser)).run input of
-                                  Success (input', parsed_string) =>  Success (input', JsonString parsed_string)
-                                | Failure err => Failure err
-                             )
+  jsonString_parser =
+  Parser (λ input.
+            case (special_char_parser <&> (normal_string_parser <&> special_char_parser)).run input of
+              Success (input', parsed_string) =>  Success (input', String (strlit parsed_string))
+            | Failure err => Failure err
+         )
 End
 
-
+   
 
 (* Array parser *)
 
 (* Consumes a compulsory single comma *)
 Definition comma_parser_def:
-  comma_parser = const_parser "" (char_parser #",")
+  comma_parser = "" <x> (char_parser #",")
 End    
         
 (* consumes a compulsory single comma surrounded by optional whitespaces. E.g.: "     ,     "  *)
-Definition separator_parser_def:
-  separator_parser = (many_whitespace_parser <&> (comma_parser <&> many_whitespace_parser))
-End
-        
-Definition open_bracket_parser_def:
-  open_bracket_parser = (many_whitespace_parser <&> ((const_parser "" (char_parser #"[")) <&> many_whitespace_parser))
+Definition comma_separator_parser_def:
+  comma_separator_parser = (many_whitespace_parser <&> (comma_parser <&> many_whitespace_parser))
 End
 
+(* parses some values separated by comma and collects them in a list *)
+Definition array_recursive_parser_def[tailrecursive]:
+  array_recursive_parser p output =
+  case output of
+    Success (input, previously_parsed) =>
+      (case p input of
+         Success (input1, parsed_element) =>
+           (case comma_separator_parser.run input1 of     
+              Success (input2, _) => array_recursive_parser p (Success (input2, (previously_parsed ++ [parsed_element])))
+            | Failure _ => Success (input1, (previously_parsed ++ [parsed_element])))
+       | Failure _ => output)
+  | Failure e => Failure e
+End
+
+(* parser of simple json values *)
+Definition jsonSimple_parser_def:
+  jsonSimple_parser = jsonBool_parser <|> jsonNull_parser <|> jsonNumber_parser <|> jsonString_parser
+End
+
+        
+Theorem jsonSimple_parser_length_thm:
+  ∀ input input' parsed. jsonSimple_parser.run input = Success(input', parsed) ⇒ STRLEN(input'.String) < STRLEN(input.String)
+Proof
+  cheat
+QED
+    
+
+Definition open_bracket_parser_def:
+  open_bracket_parser = Parser(λinput.
+  case (many_whitespace_parser <&> (("" <x> (char_parser #"[")) <&> many_whitespace_parser)).run input of
+    Success (input', parsed) => Success(input', [])
+  | Failure e => Failure e)
+End
+
+
+Theorem open_bracket_parser_length_thm:
+  ∀ input input' parsed. open_bracket_parser.run input = Success(input', parsed) ⇒ STRLEN(input'.String) < STRLEN(input.String)
+Proof
+  cheat
+QED
+    
+
+        
 Definition closed_bracket_parser_def:
-  closed_bracket_parser = (many_whitespace_parser <&> ((const_parser "" (char_parser #"]")) <&> many_whitespace_parser))
-End  
+  closed_bracket_parser = Parser(λinput.
+  case (many_whitespace_parser <&> (("" <x> (char_parser #"]")) <&> many_whitespace_parser)).run input of
+    Success (input', parsed) => Success(input', [])
+  | Failure e => Failure e)
+End
+
+
+Theorem closed_bracket_parser_length_thm:
+  ∀ input input' parsed. closed_bracket_parser.run input = Success(input', parsed) ⇒ STRLEN(input'.String) < STRLEN(input.String)
+Proof
+  cheat
+QED
+    
+
+
+(* Working New version *)
+Definition jsonArray_parser_def:
+  jsonArray_parser element_parser input =
+           let p = closed_bracket_parser <&> Parser(λ x. (array_recursive_parser element_parser (open_bracket_parser.run x)))
+           in
+             case p.run input of
+               Success (input1, parsed_list) => Success (input1, (Array parsed_list))
+             | Failure e => Failure e
+End   
+
+
+
+Theorem jsonArray_parser_length_thm:
+  ∀ input input' parsed parser. jsonArray_parser parser  input = Success(input', parsed) ⇒ STRLEN(input'.String) < STRLEN(input.String)
+Proof
+  cheat
+QED
+    
+     
+
+(* Working version Working do  not touch*)
+Definition jsonValue_parser_def:
+  jsonValue_parser input = (jsonSimple_parser <|> Parser(jsonArray_parser jsonValue_parser)).run input
+Termination
+  cheat
+End
+
+
+EVAL“jsonValue_parser (Input 0 "[[[null]]]")”;
+EVAL“jsonValue_parser (Input 0 "5")”;
+EVAL“jsonValue_parser (Input 0 "[null, true, false, 44]")”;        
+
+ 
+  
+
+(* Trying to prove termination *)
+Definition jsonValue_parser_def:
+  jsonValue_parser input = (jsonSimple_parser <|> Parser(jsonArray_parser jsonValue_parser)).run input
+End
+        
+Termination
+  cheat
+End
+ 
+Termination
+  WF_REL_TAC ‘measure (λ input. LENGTH input.String)’ >>
+  rw[]>>
+End
+
+
+      
 
 (* Consumes a compulsory single colon *)
 Definition colon_parser_def:
-  colon_parser = const_parser "" (char_parser #":")
+  colon_parser = "" <x> (char_parser #":")
 End
 
+
+Theorem colon_parser_length_thm:
+  ∀ input input' parsed. colon_parser.run input = Success(input', parsed) ⇒ STRLEN(input'.String) < STRLEN(input.String)
+Proof
+  cheat
+QED
+    
+        
+
+  (*      
 Definition open_brace_parser_def:
-  open_brace_parser = (many_whitespace_parser <&> ((const_parser "" (char_parser #"{")) <&> many_whitespace_parser))
+  open_brace_parser = (many_whitespace_parser <&> (("" <x> (char_parser #"{")) <&> many_whitespace_parser))
 End
 
 Definition closed_brace_parser_def:
-  closed_brace_parser = (many_whitespace_parser <&> ((const_parser "" (char_parser #"}")) <&> many_whitespace_parser))
+  closed_brace_parser = (many_whitespace_parser <&> (("" <x> (char_parser #"}")) <&> many_whitespace_parser))
+End
+*)
+
+
+Definition open_brace_parser_def:
+  open_brace_parser = Parser(λinput.
+  case (many_whitespace_parser <&> (("" <x> (char_parser #"{")) <&> many_whitespace_parser)).run input of
+    Success (input', parsed) => Success(input', [])
+  | Failure e => Failure e)
 End
 
+
+Theorem open_brace_parser_length_thm:
+  ∀ input input' parsed. open_brace_parser.run input = Success(input', parsed) ⇒ STRLEN(input'.String) < STRLEN(input.String)
+Proof
+  cheat
+QED
+    
+        
+Definition closed_brace_parser_def:
+  closed_brace_parser = Parser(λinput.
+  case (many_whitespace_parser <&> (("" <x> (char_parser #"}")) <&> many_whitespace_parser)).run input of
+    Success (input', parsed) => Success(input', [])
+  | Failure e => Failure e)
+End
+
+
+Theorem closed_brace_parser_length_thm:
+  ∀ input input' parsed. closed_brace_parser.run input = Success(input', parsed) ⇒ STRLEN(input'.String) < STRLEN(input.String)
+Proof
+  cheat
+QED
+    
+        
+        
 Definition separator_colon_parser_def:
   separator_colon_parser =  (many_whitespace_parser <&> (colon_parser <&> many_whitespace_parser))
 End
 
 
 
-Definition jsonValue_parser_components_def:
-  (jsonValue_parser_precursor input =  (jsonBool_parser <|> jsonNull_parser <|> jsonNumber_parser <|> jsonString_parser <|> (Parser(jsonArray_parser_precursor)) <|> (Parser(jsnObject_parser_precursor))).run input) ∧
+Theorem separator_colon_parser_length_thm:
+  ∀ input input' parsed. separator_colon_parser.run input = Success(input', parsed) ⇒ STRLEN(input'.String) < STRLEN(input.String)
+Proof
+  cheat
+QED
+    
+        
 
-(array_recursive_helper input accumulator =
- case (jsonValue_parser_precursor input) of
-   Success (input', parsed) =>
-     (let accumulator' = accumulator ++ [parsed]
-      in case separator_parser.run input' of     
-           Success (input'', _) =>
-             array_recursive_helper input'' accumulator'
-         | Failure _ =>
-             Success (input', accumulator'))
- | Failure _ =>
-     Success (input, accumulator)) ∧
+EVAL“(separator_colon_parser <&> stringliteral_parser).run (Input 0 "\"my-key\":")”;
+type_of“jsonSimple_parser”;
+type_of“separator_colon_parser <&> stringliteral_parser”;
 
-(jsonArray_parser_precursor input = case open_bracket_parser.run input of
-                                 Success (input', _) =>
-                                   (case (array_recursive_helper input' []) of
-                                      Success (input'', parsed'') =>
-                                        (case closed_bracket_parser.run input'' of
-                                           Success (input''', _) => Success (input''', JsonArray parsed'')
-                                         | Failure _ => Failure (ParserError input''.Location ("Expected ']', but found '" ++ input''.String ++ "'")))
-                                    | Failure _ => Failure (ParserError input'.Location ("Expected json value, but found '" ++ input'.String ++ "'")))
-                                    | Failure _ => Failure (ParserError input.Location ("Expected '[', but found '" ++ input.String ++ "'"))) ∧
-                                
-(dictionary_helper input = case (separator_colon_parser <&> stringliteral_parser).run input of
+
+Definition dictionary_entry_parser_def:
+dictionary_entry_parser value_parser = Parser(λ input. case (separator_colon_parser <&> stringliteral_parser).run input of
                               Success (input',parsed') =>
                                 (
-                                case jsonValue_parser_precursor input' of
-                                  Success (input'', parsed'') => Success (input'', (parsed', parsed''))
+                                case value_parser input' of
+                                  Success (input'', parsed'') => Success (input'', ((strlit parsed'), parsed''))
                                 | Failure e => Failure e
                                 )
-                            | Failure e => Failure e) ∧
-
-(dictionary_recursive_helper input accumulator =
- case (dictionary_helper input) of
-   Success (input', parsed) =>
-     (
-     let accumulator' = accumulator ++ [parsed]
-     in
-       case separator_parser.run input' of
-         Success (input'', _) =>
-           dictionary_recursive_helper input'' accumulator'
-       | Failure _ =>
-           Success (input', accumulator')
-     )
- | Failure _ =>
-     Success (input, accumulator)) ∧
+                          | Failure e => Failure e)
+End
 
 
-(jsnObject_parser_precursor input = case open_brace_parser.run input of
 
-                                 (* found "{" *)
-                                 Success (input', _) =>
+Theorem dictionary_entry_parser_length_thm:
+  ∀ input input' parsed parser. (dictionary_entry_parser parser).run input = Success(input', parsed) ⇒ STRLEN(input'.String) < STRLEN(input.String)
+Proof
+  cheat
+QED
+    
 
-                                   (* try to parse list of json-pairs *)
-                                   (case (dictionary_recursive_helper input' []) of
 
-                                      (* found list of json-pairs *)
-                                      Success (input'', parsed'') =>
+        
+type_of“array_recursive_parser”;
+type_of“(dictionary_entry_parser jsonValue_parser).run”;
+type_of“jsonValue_parser”;
+type_of“(dictionary_entry_parser jsonValue_parser).run”;
+type_of“array_recursive_parser (dictionary_entry_parser jsonValue_parser).run ”;
+EVAL“(dictionary_entry_parser jsonValue_parser).run (Input 0 "\"my-key-1\":true,\"my-key-2\":false ")”;
+EVAL“array_recursive_parser ((dictionary_entry_parser jsonValue_parser).run) (Success ((Input 0 "\"my-key-1\":true,\"my-key-2\":false "),[]))”;
+type_of“array_recursive_parser ((dictionary_entry_parser jsonValue_parser).run) (Success ((Input 0 "\"my-key-1\":true,\"my-key-2\":false "),[]))”;
 
-                                        (* try to parse "}" *)
-                                        (case closed_brace_parser.run input'' of
 
-                                           (* found "}" *)
-                                           Success (input''', _) => Success (input''', JsonObject parsed'')
+(* Compiles New version *)
+Definition jsonDictionary_parser_def:
+  jsonDictionary_parser value_parser input =
+  let p =
+      closed_brace_parser <&> Parser(λ x. (array_recursive_parser ((dictionary_entry_parser value_parser).run) (open_brace_parser.run x)))
+  in
+    case p.run input of
+      Success (input1, parsed_list) => Success (input1, (Object parsed_list))
+    | Failure e => Failure e
+End
 
-                                         (* did not find "]"*)
-                                         | Failure _ => Failure (ParserError input''.Location ("Expected ']', but found '" ++ input''.String ++ "'")))
 
-                                    (* did not find json values *)
-                                    | Failure _ => Failure (ParserError input'.Location ("Expected json value, but found '" ++ input'.String ++ "'")))
 
-                               (* did not find "[" *)
-                                    | Failure _ => Failure (ParserError input.Location ("Expected '[', but found '" ++ input.String ++ "'")))
+Theorem jsonDictionary_parser_length_thm:
+  ∀ input input' parsed parser. jsonDictionary_parser parser  input = Success(input', parsed) ⇒ STRLEN(input'.String) < STRLEN(input.String)
+Proof
+  cheat
+QED
+         
+
+EVAL“(jsonDictionary_parser jsonValue_parser).run (Input 0 "\"my-key-1\":true,\"my-key-2\":false ") ”;
+type_of“jsonDictionary_parser”;
+type_of“jsonValue_parser”;
+type_of“jsonDictionary_parser jsonValue_parser”;
+
+
+Definition input_size_def:
+  input_size (Input loc str) = LENGTH str
+End
+
+Termination
+
+  WF_REL_TAC ‘measure input_size’ >>
+  rw[]>>
+        
+   Cases_on ‘input’>|
+   fs [input_size_def]>>
+   imp_res_tac open_bracket_parser_decreases_input
+   \\ imp_res_tac array_recursive_parser_decreases_input
+   \\ decide_tac)
+                                 
+
+(* Working version Working do  not touch*)
+Definition jsonValue_parser_def:
+  jsonValue_parser input = (jsonSimple_parser <|> (Parser(jsonDictionary_parser jsonValue_parser)) <|> (Parser(jsonArray_parser jsonValue_parser)) ).run input
 Termination
   cheat
+End
+
+EVAL“jsonValue_parser (Input 0 "{\"key\":1}")”
+EVAL“jsonValue_parser (Input 0 "[{\"my-key-1\":true,\"my-key-2\":[false, null, {\"kkk\":-10}, 0x11, [] ]}, {}, {}, []]") ”;
+
+
+
+Theorem jsonValue_parser_length_thm:
+  ∀ input input' parsed any_parser. any_parser = (jsonSimple_parser <|> (Parser(jsonDictionary_parser jsonValue_parser)) <|> (Parser(jsonArray_parser any_parser))) ∧
+  any_parser.run input = Success(input', parsed) ⇒ STRLEN(input'.String) < STRLEN(input.String)
+Proof
+  cheat
+QED
+       
+
+
+
+
+                      
+
+
+Definition jsonValue_parser_def:
+  jsonValue_parser input = (jsonSimple_parser <|> (Parser(jsonDictionary_parser jsonValue_parser)) <|> (Parser(jsonArray_parser jsonValue_parser)) ).run input
+End
+Termination
+  
+  (* Establish the measure function based on input length *)
+  WF_REL_TAC ‘measure (λ input. LENGTH input.String)’ >>
+
+  (* Case split for alternative parser *)
+  Cases_on ‘jsonSimple_parser.run input’ THENL
+
+  [
+    (* Case 1: jsonSimple_parser is successful *)
+    rw[jsonSimple_parser_length_thm] THEN
+    meson_tac[]>>
+
+    
+        
+Termination
+  WF_REL_TAC ‘measure (λ input. LENGTH input.String)’ >>
+  rw[alt_parser_length_thm, jsonSimple_parser_length_thm, jsonArray_parser_length_thm, jsonDictionary_parser_length_thm]>>
 End
 
 
 
 
+Definition parser1_def:
+  parser1 input = Parser(simple_json_parser) <|> 
+  let p2 = λx. case simple_json_parser x of Success s => Success s | _ => parser1 x
+      in array_parser_builder p2 input                                                               
+Termination
+  cheat
+End
+
+   
+Definition parser1_def:
+  parser1 input =
+  let p2 = λx. case simple_json_parser x of Success s => Success s | _ => parser1 x
+      in array_parser_builder p2 input                                                               
+Termination
+  cheat
+End
+Termination
+  rw[]>>
+  WF_REL_TAC ‘measure (λx input. LENGTH input.String
+                           | INR input => LENGTH input.String)’ >>
+End
+
+EVAL“parser1 (Input 0 "[[[null]]]")”;
+EVAL“parser1 (Input 0 "5")”;
+EVAL“parser1 (Input 0 "[null, true, false, 44]")”;
+
+
+
+        
+
+Termination
+  fs[]>>
+  WF_REL_TAC ‘measure (λx. case x of
+                             INL input => LENGTH input.String
+                           | INR input => LENGTH input.String)’ >>
+  rw[]>>
+
+         
+        
+(* TRY make it tailrecursive by introducin an inner recursive lambda function *)
+(* TRY to introduce empty string exit immediately in parser *)
+  
+(* Experiment: measure works, proof is not finished *)
+Definition parser1_def:
+  parser1 input =
+   let p2 = λx. case parserC x of Success s => Success s | _ => parser1 input 
+   in
+     case parserOR parserB (parserOR p2 parserA) input of
+       Success (input', parsed) =>  Success (input', parsed)
+     | Failure e => Failure e
+End
+WF_REL_TAC ‘measure (λx. LENGTH x.String)’ >>
+           rw[]>>
+
+
+(* Experiment: measure works, proof is not finished don't touch*)
+Definition example_def:
+  (parser1 input = case parserOR parserB (parserOR parser2 parserA) input of
+                     Success (input', parsed) =>
+                       let f = λx. x in Success (input', f(parsed))
+                     | Failure e => Failure e
+  ) ∧
+
+  (parser2 input = case parserC input of
+                     Failure e => parser1 input
+                   | s => s
+  ) 
+End
+Termination
+  WF_REL_TAC ‘measure (λx. case x of
+                             INL input => LENGTH input.String
+                           | INR input => LENGTH input.String)’ >>
+  rw[]>>
+                 
+End
+
+
+Definition jsonArray_recursive_parser_precursor_def:
+  jsonArray_recursive_parser_precursor input = (jsonBool_parser <|>
+jsonNull_parser <|> jsonNumber_parser <|> jsonString_parser <|> (jsonArray_parser Parser(jsonArray_recursive_parser_precursor))).run input          
+End
+Termination
+  rw[]>>
+    WF_REL_TAC ‘measure (λinput. LENGTH input.String)’ >>
+(*  ∃R. WF R ∧ ∀input a. R a input: proof *)
+
+                       
+        
+EVAL“open_bracket_parser.run (Input 0 "[123")”;
+
+type_of“open_bracket_parser”;
+type_of“simple_json_parser”;
+type_of“open_bracket_parser <&> open_bracket_parser”;
+        
+
 
 (* SIMPLIFIED TRIAL *)
+  
 
 Definition jsonValue_parser_components_def:
   (jsonValue_parser_precursor input =  (jsonBool_parser <|> jsonNull_parser <|> jsonNumber_parser <|> jsonString_parser <|> (Parser(jsonArray_parser_precursor))).run input) ∧
@@ -697,17 +1204,71 @@ Definition jsonValue_parser_components_def:
                                    (case (array_recursive_helper input' []) of
                                       Success (input'', parsed'') =>
                                         (case closed_bracket_parser.run input'' of
-                                           Success (input''', _) => Success (input''', JsonArray parsed'')
+                                           Success (input''', _) => Success (input''', Array parsed'')
                                          | Failure _ => Failure (ParserError input''.Location ("Expected ']', but found '" ++ input''.String ++ "'")))
                                     | Failure _ => Failure (ParserError input'.Location ("Expected json value, but found '" ++ input'.String ++ "'")))
                                     | Failure _ => Failure (ParserError input.Location ("Expected '[', but found '" ++ input.String ++ "'"))) 
 
+End
+
 Termination
-  cheat
+  WF_REL_TAC ‘measure (λx. case x of
+                             INL input => LENGTH input.String
+                           | INR input => LENGTH input.String)’ >>
+  fs[LENGTH_TL]
 End
 
 
- 
+Definition simple_json_parser_def:
+  simple_json_parser = jsonBool_parser <|> jsonNull_parser <|> jsonNumber_parser <|> jsonString_parser
+End
+        
+
+(* MODIFIED SIMPLIFIED TRIAL *)
+  
+
+Definition jsonValue_parser_components_def:
+
+(array_recursive_helper input accumulator =
+ case ((simple_json_parser <|> Parser(jsonArray_parser_precursor)).run input)of
+   Success (input', parsed) =>
+     (let accumulator' = accumulator ++ [parsed]
+      in case separator_parser.run input' of     
+           Success (input'', _) =>
+             array_recursive_helper input'' accumulator'
+         | Failure _ =>
+             Success (input', accumulator'))
+ | Failure _ =>
+     Success (input, accumulator)) ∧
+
+(jsonArray_parser_precursor input = case open_bracket_parser.run input of
+                                 Success (input', _) =>
+                                   (case (array_recursive_helper input' []) of
+                                      Success (input'', parsed'') =>
+                                        (case closed_bracket_parser.run input'' of
+                                           Success (input''', _) => Success (input''', Array parsed'')
+                                         | Failure _ => Failure (ParserError input''.Location ("Expected ']', but found '" ++ input''.String ++ "'")))
+                                    | Failure _ => Failure (ParserError input'.Location ("Expected json value, but found '" ++ input'.String ++ "'")))
+                                    | Failure _ => Failure (ParserError input.Location ("Expected '[', but found '" ++ input.String ++ "'"))) 
+
+End
+
+Termination
+  WF_REL_TAC ‘measure (λx. case x of
+                             INL input => LENGTH input.String
+                           | INR input => LENGTH input.String)’ >>
+  fs[LENGTH_TL]
+End
+
+
+        
+
+type_of“INR”;
+type_of“INL”;
+type_of“OUTR”;
+type_of“OUTL”;
+
+
 
 (* requires jsonValue_parser_precursor*)
 Definition jsonValue_parser_def:
@@ -719,8 +1280,41 @@ Definition jsonValue_parser_def:
                                        )
                            )
 End
-  
 
+
+Definition mlstring_list_to_string_def:
+  (mlstring_list_to_string (List []) = "") ∧
+  (mlstring_list_to_string (List ((strlit s)::xs)) = 
+    s ++ mlstring_list_to_string (List xs)) ∧
+  (mlstring_list_to_string (Append l1 l2) = 
+    mlstring_list_to_string l1 ++ mlstring_list_to_string l2) ∧
+  (mlstring_list_to_string Nil = "")
+End
+        
+
+Definition json_to_string_def:
+  json_to_string json = mlstring_list_to_string (json_to_mlstring json)
+End
+
+
+       
+EVAL“json_to_string (Object [(strlit "my-key", Null)])”;
+EVAL“jsonValue_parser.run (Input 0 (json_to_string (Object [(strlit "my-key", Null)])))”;
+
+(* CORRECTNESS EXAMPLE *)                         
+EVAL“(Object [(strlit "my-key", Null)]) = THE(extract((jsonValue_parser.run (Input 0 (json_to_string (Object [(strlit "my-key", Null)]))))))”;
+
+
+Theorem parser_correctness_thm:
+  ∀json. THE(extract(jsonValue_parser.run (Input 0 (json_to_string json)))) = json
+Proof
+  rw[json_to_string_def, jsonValue_parser_def, extract_def]>>
+                           fs[json_to_string_def; jsonValue_parser_def; extract_def]>>
+QED
+                   
+type_of“THE”;
+
+                   
 val _ = export_theory();      
 
 
@@ -743,18 +1337,22 @@ EVAL“jsonValue_parser.run (Input 0 ("false"))”;
 EVAL“jsonValue_parser.run (Input 0 ("[{\"key-1\": [\"100\", 100, true]}, {\"key-2\": \"value\"}]"))”;
 EVAL“jsonValue_parser.run (Input 0 ([CHR 34] ++ "mystring" ++ [CHR 34]))”;
 EVAL“jsonValue_parser.run (Input 0 "[1, [null, []],[],[true, \"my_string\" ],false, ]")”;
-
 EVAL“jsonValue_parser.run (Input 0 "[{}]")”;
 EVAL“jsonValue_parser.run (Input 0 "[{},{},{}]")”;
 EVAL“jsonValue_parser.run (Input 0 "[{ \"key-1\" : { \"key-2\" : { \"key-3\" : [] } }}]")”;
+EVAL“jsonValue_parser.run (Input 0 ("[-1, true, -123]"))”;
 
 
 (* FAIL TESTS *)
 EVAL“ jsonValue_parser.run (Input 0 ([CHR 34] ++ "normal string" ++ [CHR 34] ++ "another_normal_string"))”;
 EVAL“ jsonValue_parser.run (Input 0 ("[1, true123]"))”;
 
-      
-      
+type_of“json_to_mlstring Null”;
+type_of“json_to_mlstring”;
+EVAL“json_to_mlstring Null”;
+EVAL“json_to_mlstring Null”;
+EVAL“json_to_mlstring Bool true”;
+EVAL“json_to_mlstring Bool false”;
 
 (* MUTUALLY RECURSIVE DEFINITION EXAMPLE *)
 
@@ -779,29 +1377,492 @@ Definition or_def:
                         |NONE => p2 x
 End
 
-(* Experiment [tailrecursive] *)
+        
+
 Definition example_def:
   (comb s = or (or (fc 5) (fc 7)) foo s) ∧
         
   (helper s acc =                                                                                       
    if comb s = NONE then acc else helper (TL s) (1 + acc)) ∧
-
-   (helper1 x = helper x 0) ∧
    
   (foo x = case fc 0 x of
            | NONE => NONE
-           | SOME _ => SOME (1 + helper1 (TL x)))
+           | SOME _ => SOME (1 + (helper (TL x) 0)))
+End
 Termination
-  cheat
+  WF_REL_TAC ‘measure (λx. case x of
+                             INL x => LENGTH x.String
+                           | INR x => LENGTH x.String)’ >>
+  fs[LENGTH_TL]>>
+
+
+
+        
+  WF_REL_TAC ‘inv_image ($< LEX $<) (λx. case x of
+                INL s => (LENGTH s, 0)
+              | INR (INL (s, acc)) => (LENGTH s, acc)
+              | INR (INR s) => (LENGTH s, 0))’ >>
+  rw[] >>
+  TRY(Cases_on `OUTR (scratch$old37->example_def_UNION_aux<-old R (INL s))`) >>
+  fs[LENGTH_TL] >>
+  TRY(Cases_on `fc 0 x`) >>
+  fs[] >>
+  decide_tac
 End
 
+
+Termination
+  WF_REL_TAC `inv_image ($< LEX $<) (λx. case x of
+                INL s => (LENGTH s, 0)
+              | INR (INL (s, acc)) => (LENGTH s, acc)
+              | INR (INR s) => (LENGTH s, 0))` >>
+  rw[] >>
+
+  fs[LENGTH_TL] >>
+  TRY(Cases_on `fc 0 x`) >>
+  fs[] >>
+  metis_tac[LESS_EQ_LESS_TRANS, LESS_TRANS, NOT_LESS, LESS_OR_EQ]
+End
+        
+
+(* Parsing a list of numbers [tailrecursive]: works*)
+Definition example_def:
+  (parse1 acc s = case s of
+                    [] => acc
+                  | l =>
+                      (case (HD l) of
+                         #"A" => parse2 (1 + acc) (TL l)
+                       | _ => parse1 (2 + acc) (TL l)
+                      )
+
+  ) ∧
+
+  (parse2 acc s = case s of
+                    [] => acc
+                  | l => parse1 (0 + acc) (TL l))
+End
+
+Termination
+  WF_REL_TAC ‘measure (λx. case x of
+                             INL (_, s) => LENGTH s
+                           | INR (_, s) => LENGTH s)’ >>
+  fs[LENGTH_TL]
+                           
+End
+
+
+
+
+             
+(* Parsing a list of numbers [tailrecursive]: works. don't touch*)
+Definition example_def:
+  (parser1 input = case input.String of
+                    "" => Success (input, "")
+                  | _ =>
+                      (case (HD input.String) of
+                         #"A" => parser2 (Input (input.Location + 1) (TL input.String))
+                       | _ => parser1 (Input (input.Location + 0) (TL input.String))
+                      )
+  ) ∧
+
+  (parser2 input = case input.String of
+                    "" => Success (input, "")
+                  | _ => parser1 (Input (input.Location + 0) (TL input.String))
+  )
+End
+Termination
+  WF_REL_TAC ‘measure (λx. case x of
+                             INL input => LENGTH input.String
+                           | INR input => LENGTH input.String)’ >>
+  fs[LENGTH_TL]>>
+                           
+End
+
+
+
+Theorem parserA_length_thm:
+  ∀ input input' parsed. parserA input = Success(input', parsed) ⇒ STRLEN(input'.String) < STRLEN(input.String)
+Proof
+  cheat
+QED
+
+
+Theorem parserA_either_thm:
+  ∀ input input' parsed f. parserA input = Success(input', parsed) ⇒ parserA input ≠ Failure f
+Proof
+  cheat
+QED
+
+        
+        
+Theorem parserB_length_thm:
+  ∀ input input' parsed. parserB input = Success(input', parsed) ⇒ STRLEN(input'.String) < STRLEN(input.String)
+Proof
+  cheat
+QED
+    
+Theorem parserC_length_thm:
+  ∀ input input' parsed. parserC input = Success(input', parsed) ⇒ STRLEN(input'.String) < STRLEN(input.String)
+Proof
+  cheat
+QED
+
+Theorem parserD_length_thm:
+  ∀ input input' parsed. parserD input = Success(input', parsed) ⇒ STRLEN(input'.String) < STRLEN(input.String)
+Proof
+  cheat
+QED
+
+Definition parserAB_def:
+  parserAB input = parserOR parserA parserB input
+End
+
+Theorem parserAB_length_thm:
+  ∀ input input' parsed. parserAB input = Success(input', parsed) ⇒ STRLEN(input'.String) < STRLEN(input.String)
+Proof
+  cheat
+QED
+
+Theorem parserOR_length_thm:
+  ∀ input input' p1 p2 parsed. parserOR p1 p2 input = Success(input', parsed) ⇒ STRLEN(input'.String) < STRLEN(input.String)
+Proof
+  cheat
+QED
+
+Theorem parserAND_length_thm:
+  ∀ input input' p1 p2 parsed. parserAND p1 p2 input = Success(input', parsed) ⇒ STRLEN(input'.String) < STRLEN(input.String)
+Proof
+  cheat
+QED        
+
+
+(* Experiment: measure works, proof is not finished *)
+Definition example_def:
+  (parser1 input = case parserA input of
+                     Success (input', parsed) => parser2 input'
+                   | _ => parser1 input
+  ) ∧
+
+  (parser2 input = case parserB input of
+                     Success (input', parsed) => parser1 input'
+                   | _ => Success (input, "")
+  ) 
+End
+Termination
+  WF_REL_TAC ‘measure (λx. case x of
+                             INL input => LENGTH input.String
+                           | INR input => LENGTH input.String)’ >>
+                 
+End
+
+
+(* Experiment: measure works, proof is not finished *)
+Definition example_def:
+  (parser1 input = case parserOR parserA parserB input of
+                     Success (input', parsed) => parser2 input'
+                   | _ => parser1 input
+  ) ∧
+
+  (parser2 input = case parserAND parserC parserD input of
+                     Success (input', parsed) => parser1 input'
+                   | _ => Success (input, "")
+  ) 
+End
+
+Termination
+  WF_REL_TAC ‘measure (λx. case x of
+                             INL input => LENGTH input.String
+                           | INR input => LENGTH input.String)’ >>
+                 
+End
+
+(* Experiment: measure works, proof is not finished *)
+Definition example_def:
+  (parser1 input = case parserOR parser3 (parserOR parserA parserB) input of
+                     Success (input', parsed) => parser2 input'
+                   | _ => parser1 input
+  ) ∧
+
+  (parser2 input = case parserAND parserC parserD input of
+                     Success (input', parsed) => parser1 input'
+                   | _ => Success (input, "")
+  ) 
+End
+
+Termination
+  WF_REL_TAC ‘measure (λx. case x of
+                             INL input => LENGTH input.String
+                           | INR input => LENGTH input.String)’ >>
+                 
+End
+
+
+(*
+   ∃R. WF R ∧ (∀input a. R (INL a) (INR input)) ∧
+       ∀input e.
+         simple_json_parser input = Failure e ⇒ R (INR input) (INL input)
+   
+   : proof
+*)
+
+        
+             
+(* Parsing a list of numbers*)
+Definition example_def:
+  (parser1 input = parserOR parserAB parser3 input
+  ) ∧
+
+  (parser2 input = case parser1 input of
+                    Success (input', parsed) => parser1 input'
+                  | _ => Success (input, "") 
+  ) ∧
+
+  (parser3 input = parserAND parserC parser2 input
+  )
+End
+Termination
+  WF_REL_TAC ‘measure (λx. case x of
+                             INL input => LENGTH input.String
+                           | INR input => LENGTH input.String)’ >>
+  fs[parserA_length_thm]>>
+  fs[parserB_length_thm]>>                        
+End
+
+
+
+        
+
+Definition jsonValue_parser_components_def:
+  (jsonValue_parser_precursor input =  parserOR parserA parserB input ∧
+
+(array_recursive_helper input =
+ case (jsonValue_parser_precursor input) of
+   Success (input', parsed) =>
+     (let accumulator' = accumulator ++ [parsed]
+      in case separator_parser.run input' of     
+           Success (input'', _) =>
+             array_recursive_helper input'' accumulator'
+         | Failure _ =>
+             Success (input', accumulator'))
+ | Failure _ =>
+     Success (input, accumulator)) ∧
+
+(jsonArray_parser_precursor input = case open_bracket_parser.run input of
+                                 Success (input', _) =>
+                                   (case (array_recursive_helper input' []) of
+                                      Success (input'', parsed'') =>
+                                        (case closed_bracket_parser.run input'' of
+                                           Success (input''', _) => Success (input''', Array parsed'')
+                                         | Failure _ => Failure (ParserError input''.Location ("Expected ']', but found '" ++ input''.String ++ "'")))
+                                    | Failure _ => Failure (ParserError input'.Location ("Expected json value, but found '" ++ input'.String ++ "'")))
+                                    | Failure _ => Failure (ParserError input.Location ("Expected '[', but found '" ++ input.String ++ "'"))) 
+
+End
+Termination
+  WF_REL_TAC ‘measure (λx. case x of
+                             INL input => LENGTH input.String
+                           | INR input => LENGTH input.String)’ >>
+  fs[LENGTH_TL]
+End
+(* Parsing a list of numbers *)
+Definition example_def:
+        
+  (parser1 input = case input.String of
+                    "" => Success (input, "")
+                  | _ =>
+                      (case (parserOR parserA parserB input) of
+                         Success _ => parser2 (Input (input.Location + 1) (TL input.String))
+                       | _ => parser1 (Input (input.Location + 0) (TL input.String))
+                      )
+  ) ∧
+
+  (parser2 input = case input.String of
+                    "" => Success (input, "")
+                  | _ => parserAND parserA parser1 (Input (input.Location + 0) (TL input.String))
+  )
+End
+Termination
+  WF_REL_TAC ‘measure (λx. case x of
+                             INL input => LENGTH input.String
+                           | INR input => LENGTH input.String)’ >>
+  fs[LENGTH_TL]>>
+  rw[SUC_LESS]>>
+                           
+End
+
+
+
+EVAL“SUC_LESS”;
+
+
+
+        
+
+Definition parserA_def:
+  parserA input = case input.String of
+                     "" => Failure (ParserError input.Location "Error in parser A: Empty input")
+                   | _ =>
+                       (case (HD input.String) of
+                          #"A" => Success ((Input (input.Location + 1) (TL input.String)), "A")
+                        | _ => Failure (ParserError input.Location  "Error in parser A but did not get it")
+                      )
+End
+        
+
+Definition parserB_def:
+  parserB input = case input.String of
+                     "" => Failure (ParserError input.Location "Error in parser B: Empty input")
+                   | _ =>
+                       (case (HD input.String) of
+                          #"B" => Success ((Input (input.Location + 1) (TL input.String)), "B")
+                        | _ => Failure (ParserError input.Location  "Error in parser B but did not get it")
+                      )
+End
+
+
+Definition parserC_def:
+  parserC input = case input.String of
+                     "" => Failure (ParserError input.Location "Error in parser C: Empty input")
+                   | _ =>
+                       (case (HD input.String) of
+                          #"C" => Success ((Input (input.Location + 1) (TL input.String)), "C")
+                        | _ => Failure (ParserError input.Location  "Error in parser C but did not get it")
+                      )
+End
+
+Definition parserD_def:
+  parserD input = case input.String of
+                     "" => Failure (ParserError input.Location "Error in parser D: Empty input")
+                   | _ =>
+                       (case (HD input.String) of
+                          #"D" => Success ((Input (input.Location + 1) (TL input.String)), "D")
+                        | _ => Failure (ParserError input.Location  "Error in parser D but did not get it")
+                      )
+End
+
+
+        
+Definition parserOR_def:
+  parserOR p1 p2 input = case p1 input of
+                       Success s => Success s
+                     |_ => p2 input
+End
+
+
+Definition parserAND_def:
+  parserAND p1 p2 input = case (p1 input) of
+                            Success (input', parsed) =>
+                              (case p2 input' of
+                                Success (input'', parsed') =>  Success (input'', "")
+                              | Failure f => Failure f)
+                          | Failure f => Failure f
+End
+
+
+
+Definition example_def:
+(parser1 input = parserOR (parserOR parserA parserB) (parser3) input) ∧
+           
+(parser2 input = parserAND parser1 parser2 input) ∧
+         
+(parser3 input = case input.String of
+                    "" => Success (input, "")
+                  | _ => parser2 input
+)
+End      
+Termination
+  WF_REL_TAC ‘measure (λx. case x of
+                           | INL input => LENGTH input.String
+                           | INR input => LENGTH input.String)’ >>
+  fs[LENGTH_TL]>>
+                           
+End
+
+type_of“#"A"”;
+type_of“HD "AAA"”;  
+
+        
+   
+type_of“TL”;
+EVAL“TL_def”;
+        
+
+type_of“type_size”;
+type_of“obj_size”;
+type_of“obj1_size”;
+type_of“list_size”;
+type_of“list_size LENGTH”;
+type_of“LENGTH”;
+type_of“λx:char. 1:num”;
+type_of“list_size (λx:char. 1:num) ”;
+type_of“list_size (λx:char. 1:num) "123" ”;
+type_of“list_size (λx:char. 1:num) [] ”;
+EVAL“list_size (λx:char. 1:num) "AB" ”;
+
+
+
+        
+
+Termination
+  WF_REL_TAC ‘measure (λ(s,a).
+       | INL (s, a) => list_size (λx:char. 1:num) s
+       | INR (s, a) => list_size (λx:char. 1:num) s’>>
+End
+
+
+  (WF_REL_TAC `measure (\x. case x of
+                  INR (x,_) => type1_size x
+                | INL (x,_) => type_size x)`)
+
+val (parse1_def, parse2_def) = tDefine "parse" ‘
+  (parse1 s acc = case s of
+                    [] => acc
+                  | (l::ls) => parse2 ls (1 + acc + l)) ∧
+  (parse2 s acc = case s of
+                    [] => acc
+                  | (l::ls) => parse1 ls (2 + acc + l))’
+  (WF_REL_TAC ‘measure (λx. case x of
+                             INL (s, _) => LENGTH s
+                           | INR (s, _) => LENGTH s)’)
+
+
+val example_def =
+   ⊢ (∀s acc.
+        parse1 s acc =
+        case s of
+          [] => acc
+        | v2::v3 => parse2 (TL (v2::v3)) (1 + acc + HD (v2::v3))) ∧
+     ∀s acc.
+       parse2 s acc =
+       case s of
+         [] => acc
+       | v2::v3 => parse1 (TL (v2::v3)) (2 + acc + HD (v2::v3)): thm
+
+Initial goal:
+
+∃R. WF R ∧
+    (∀acc s v2 v3.
+       s = v2::v3 ⇒ R (INL (TL (v2::v3),2 + acc + HD (v2::v3))) (INR (s,acc))) ∧
+    ∀acc s v2 v3.
+      s = v2::v3 ⇒ R (INR (TL (v2::v3),1 + acc + HD (v2::v3))) (INL (s,acc))
+
+
+
+
+
+
+
+
+
+
+
+                
         
 (* MUTUALLY RECURSIVE DEFINITION EXAMPLE *)
 
+type_of“size”;
 
-
-open jsonLangTheory;
-open mlstringTheory;
+        
 
 type_of“json_to_mlstring”;
 EVAL“”;
@@ -810,14 +1871,45 @@ type_of“Int 3”;
 type_of“Object ([])”;
 type_of“Object ([("",Int 3)])”;
 type_of“strlit”;
-
-
 type_of“String”;
 type_of“strlit "mystring"”;
 type_of“String (strlit "mystring")”;
 
 type_of“Object ([(strlit "my-key",Int 3)])”;
 type_of“Object ([(strlit "my-key-1",Int 111); (strlit "my-key-2",Int 222)])”;
+
+               
+EVAL“json_to_mlstring Null”;
+EVAL“json_to_mlstring (Array [])”;
+EVAL“json_to_mlstring (Array [Null])”;
+EVAL“json_to_mlstring (Object [])”;
+EVAL“json_to_mlstring (Object [(strlit "my-key", Null)])”;
+EVAL“json_to_mlstring (Bool true)”;
+
+type_of“json_to_mlstring (Bool true)”;
+type_of“json_to_mlstring”;
+type_of“mlstring_list_to_string”;
+type_off“app_list”;
+
+
+
+
+EVAL“jsonValue_parser (json_to_string (Object [(strlit "my-key", Null)]))”;
+
+EVAL“json_to_mlstring (Array [])”;
+EVAL“json_to_mlstring (Array [Bool true; Bool false])”;
+EVAL“mlstring_list_to_string(json_to_mlstring (Array [Bool true; Bool false]))”;
+
+        
+
+
+
+        
+
+EVAL“json_to_mlstring (Object ([(strlit "my-key",Int 3)]))”;
+EVAL“Object ([(strlit "my-key",Int 3)])”;
+type_of“Object ([(strlit "my-key-1",Int 111); (strlit "my-key-2",Int 222)])”;           
+EVAL“json_to_mlstring (Int 3)”;
 
 (*
 
@@ -847,7 +1939,16 @@ val _ = Datatype`
 
 EVAL“JsonBool true”;
 type_of“JsonBool true”;
+
 type_of“Null”;
+type_of“Object [(strlit "my-key", Null)]”;
+type_of“Array []”;
+
+EVAL“Object [(strlit "my-key", Null)]”;
+EVAL“Object []”;
+
+EVAL“FST (HD [(strlit "my-key", Null)])”;
+EVAL“SND (HD [(strlit "my-key", Null)])”;
 
 Definition jsonObject_to_Object_def:
   jsonObject_to_Object obj = case x o
@@ -856,7 +1957,7 @@ End
 
 
 (MAP char_parser s))        
-EVAL“MAP ”
+EVAL“MAP ”;
 
 Definition inputUncons_def:
   inputUncons input =
@@ -867,6 +1968,42 @@ Definition inputUncons_def:
   else NONE
 End
 
+open jsonLangTheory;
+
+
+     
+
+Definition jsonvalue_to_obj_def:
+  jsonvalue_to_obj x = case x of
+                            
+                         JsonObject ob =>
+                           case LENGTH ob of
+                           | 0 => Object []
+                           | 1 =>
+                               let key = FST (HD ob);
+                                   value = SND (HD ob)
+                               in  () ++ jsonvalue_to_obj (Object (TL ob))
+                                        
+                                         
+                                                     
+
+                           (* if more than one pair then*)
+                           (if ((LENGTH ob) = 1) then
+                              let
+                                key = 
+                                Object tail = jsonvalue_to_obj (TL ob)
+                              in
+                                        
+                                (* convert the head manually *)
+                                Object ([((String (strlit (FST (HD ob)))), (jsonvalue_to_obj (SND(HD ob))))] ++ tail)
+                            else (Object [])
+                           )
+                       | JsonArray a => Array []
+                       | JsonString s => String (strlit s)
+                       | JsonNumber n => Int n
+                       | JsonBool b => Bool b
+                       | JsonNull => Null
+End
 
                
 Definition jsonvalue_to_obj_def:
@@ -894,9 +2031,11 @@ Definition jsonvalue_to_obj_def:
                        | JsonNull => Null
 End
 
+type_of“strlit”;
+        
 Definition jsonvalue_to_obj_def:
   jsonvalue_to_obj x = case x of
-                         JsonObject ob => Array []
+                         JsonObject ob => Object []
                        | JsonArray a => Array []
                        | JsonString s => String (strlit s)
                        | JsonNumber n => Int n
@@ -924,9 +2063,319 @@ type_of“-3: int”;
   in {}, in which case it can be viewed as a key-value store of names
   (strings) and JSON objects.
 *)
-open preamble;
-open mlintTheory;
-open mlstringTheory;
+
+Definition json_to_mlstring_def:
+  (json_to_mlstring obj = 
+    case obj of
+        | Object mems => List [strlit "{"] ++
+                concat_with (MAP mem_to_string mems) (List [strlit ","]) ++
+                List [strlit "}"]
+        | Array obs => List [strlit "["] ++
+                concat_with (MAP json_to_mlstring obs) (List [strlit ","]) ++
+                List [strlit "]"]
+       | String s => List ([strlit "\""; encode_str T s; strlit "\""])
+       | Int i => List [toString i]
+       | Bool b => if b then List [strlit "true"] else List [strlit "false"]
+       | Null => List [strlit "null"])
+  /\
+  (mem_to_string n_obj = let (n, obj) = n_obj in
+        List [strlit "\""; n; strlit "\":"] ++ json_to_mlstring obj)
+Termination
+   WF_REL_TAC `measure (\x. case x of
+       | INL obj => obj_size obj
+       | INR p => obj2_size p)` \\ rw []
+End
+
+val _ = export_theory();
+
+
+
+
+(* ---- *)
+        
+EVAL“extract_first_digits "123 000"”;
+EVAL“(char_parser #"0").run  (Input 0 "0") ”;
+type_of“extract_first_digits”;
+
+(* parser that always fails *)
+Definition fail_parser_def:
+  fail_parser = Parser (λ input. Failure (ParserError input.Location input.String))
+End
+
+Definition zero_parser_def:
+  zero_parser = const_parser (0:int) (char_parser #"0")
+End
+
+Theorem zero_parser_length_thm:
+  ∀ input input'. zero_parser.run input = Success(input', parsed) ⇒ STRLEN(input'.String) < STRLEN(input.String)
+Proof
+  rw[zero_parser_def, const_parser_def]>>
+  fs[const_parser_def]>>
+  Cases_on ‘(char_parser #"0").run input’ >|
+  [
+    fs[]
+    ,
+    fs[]>>
+    Cases_on ‘p’ >|
+    [
+      fs[]>>
+      metis_tac[char_parser_length_thm]
+    ]
+  ]
+QED
+
+Definition one_parser_def:
+  one_parser = const_parser (1:int) (char_parser #"1")
+End
+
+Theorem one_parser_length_thm:
+  ∀ input input'. one_parser.run input = Success(input', parsed) ⇒ STRLEN(input'.String) < STRLEN(input.String)
+Proof
+  rw[one_parser_def, const_parser_def]>>
+  fs[const_parser_def]>>
+  Cases_on ‘(char_parser #"1").run input’ >|
+  [
+    fs[]
+    ,
+    fs[]>>
+    Cases_on ‘p’ >|
+    [
+      fs[]>>
+      metis_tac[char_parser_length_thm]
+    ]
+  ]
+QED
+
+
+               (p1.run input = Success(input1, parsed1) ∨
+                p2.run input = Success(input2, parsed2)) ∧
+
+Theorem alt_parser_length_thm:
+  ∀ p1 p2 input.
+    p1.run input = Success(_, _) ⇒
+    (p1 <|> p2).run input = Success(_, _)
+Proof
+  rw[]>|
+  fs[alt_parser_def]>>
+  rw[]>>
+  fs[alt_parser_def]>>
+        rw[]>>
+    ,
+    rw[alt_parser_def]>>
+    gs[alt_parser_def]>>
+    Cases_on ‘p1.run input’ >|
+    [
+      fs[alt_parser_def]
+      ,
+      fs[]>>
+      rw[]>>
+        
+            
+Theorem alt_parser_length_thm:
+  ∀ p1 p2 input input1' parsed1' input2' parsed2'.
+    p1.run input = Success(input1', parsed1') ∨
+    p2.run input = Success(input2', parsed2') ⇒
+    (p1 <|> p2).run input = Success(input1', parsed1') ∨ (p1 <|> p2).run input = Success(input2', parsed2')
+Proof
+  rw[]>|
+  [
+    fs[alt_parser_def]
+    ,
+    rw[alt_parser_def]>>
+    gs[alt_parser_def]>>
+    Cases_on ‘p1.run input’ >|
+    [
+      fs[alt_parser_def]
+      ,
+      fs[]>>
+      rw[]>>
+        
+        
+                
+
+Theorem alt_parser_length_thm:
+  ∀ p1 p2 input input' parsed'. (p1 <|> p2).run input = Success(input', parsed') ⇒ STRLEN(input'.String) < STRLEN(input.String)
+Proof
+  rw[]>>
+  fs[alt_parser_def]>>
+  Cases_on ‘p1.run input’ >|
+  [
+    rw[]>>
+    fs[]>>
+    Case_on ‘Failure P0’ >|   
+
+        
+
+Definition digit_parser_def:
+  digit_parser = (zero_parser <|> one_parser)
+End
+
+        
+
+     
+
+
+Theorem digit_parser_length_thm:
+  ∀ input input'. digit_parser.run input = Success(input', parsed) ⇒ STRLEN(input'.String) < STRLEN(input.String)
+Proof
+  metis_tac[one_parser_length_thm, zero_parser_length_thm, digit_parser_def]>>
+  fs[digit_parser_def]>>
+  fs[alt_parser_def]>>
+        fs[
+  Cases_on ‘zero_parser.run input’ >|
+  [
+    fs[]>>
+    rw[one_parser_length_thm]>>
+    ,
+    Cases_on ‘Success p’ >|
+    [
+      fs[]
+    ]
+    ,
+    Cases_on ‘Success p'’ >|
+    [
+      fs[]
+    ]
+    ,
+    Cases_on ‘Success p''’ >|
+    
+        
+        
+    rw[]>>
+    rw[zero_parser_length_thm]>>
+
+  rw[zero_parser_length_thm]>>
+                       
+  metis_tac[one_parser_length_thm, zero_parser_length_thm]>>
+        
+  rw[]>>
+  fs[digit_parser_def, const_parser_def]>>
+  Cases_on ‘(char_parser #"0").run input’ >|
+  [
+    fs[]>>
+     metis_tac[char_parser_length_thm]>>
+
+        
+  fs[digit_parser_def, const_parser_def, char_parser_def ]>>
+
+  Cases_on ‘(char_parser #" ").run input’ >|
+  [
+    fs[]
+    ,
+    fs[]>>
+    Cases_on ‘p’ >|
+    [
+      fs[]>>
+      metis_tac[char_parser_length_thm]
+    ]
+  ]
+QED
+
+  
+  rw[]>>
+  fs[const_parser_def]>>
+  Cases_on ‘(char_parser c).run input’ >|
+  [
+    fs[]
+    ,
+    fs[]>>
+    Cases_on ‘p’ >|
+    [
+      fs[]>>
+      metis_tac[char_parser_length_thm]
+    ]
+  ]
+QED
+
+
+EVAL“THE (extract(( (const_parser (0:int) (char_parser #"0")) <|> (const_parser (1:int) (char_parser #"1")) ).run (Input 0 "0Something-Else")))”;
+EVAL“THE (extract(( (const_parser (0:int) (char_parser #"0")) <|> (const_parser (1:int) (char_parser #"1")) ).run (Input 0 "1Something-Else")))”;
+
+EVAL“THE (extract(didgit_parser.run (Input 0 "0")))”;
+EVAL“THE (extract(didgit_parser.run (Input 0 "1")))”;
+EVAL“THE (extract(didgit_parser.run (Input 0 "2")))”;
+EVAL“THE (extract(didgit_parser.run (Input 0 "3")))”;
+EVAL“THE (extract(didgit_parser.run (Input 0 "4")))”;
+EVAL“THE (extract(didgit_parser.run (Input 0 "5")))”;
+EVAL“THE (extract(didgit_parser.run (Input 0 "6")))”;
+EVAL“THE (extract(didgit_parser.run (Input 0 "7")))”;
+EVAL“THE (extract(didgit_parser.run (Input 0 "8")))”;
+EVAL“THE (extract(didgit_parser.run (Input 0 "9")))”;
+EVAL“didgit_parser.run (Input 0 "X")”;
+EVAL“didgit_parser.run (Input 0 "")”;
+
+         
+     
+
+EVAL“THE (extract(digit_parser.run (Input 0 "0123x")))”;
+EVAL“digit_parser.run (Input 0 "0123x")”;
+type_of“digit_parser.run”;
+EVAL“0 + 10 ** 3 * 0 + 10 ** 2 * 1 + 10 ** 1 * 2 + 10 ** 0 * 3”;
+EVAL“THE (extract(digit_parser_joiner (Success ((Input 0 "0123"), 0:int))))”;
+EVAL“0 + 10 ** 0 * 2”;
+EVAL“0 + 10 ** 0 * 1”;
+EVAL“0 + 10 ** 0 * 0”;
+EVAL“ 0 + 10 ** 1 * 1 + 10 ** 0 * 2”;
+EVAL“ 0 + 10 ** 2 * 1 + 10 ** 1 * 2 + 10 ** 0 * 3”;
+EVAL“ 0 + 10 ** 3 * 0 + 10 ** 2 * 1 + 10 ** 1 * 2 + 10 ** 0 * 3”;
+
+          
+Definition character_parser_def:
+  character_parser c v = (λ x. if c = x then SOME v else NONE)                                              
+End
+
+Definition zero_parser_def:
+  zero_parser = const_parser "" (char_parser #" ")
+End
+
+     
+
+type_of“(character_parser #"0" (0:int))”
+EVAL“(character_parser #"0" (0:int)) #"0"”;
+EVAL“-1 * (THE ((character_parser #"1" (1:int)) #"1"))”;
+type_of“-1 * (THE ((character_parser #"1" (1:int)) #"1"))”;     
+
+
+
+(* assume the input is a string of digints with optional leading minus *)
+Definition toInt_def:
+  toInt s = if (first_is_minus s) then 0-t
+End
+
+Definition toInt_def:
+  toInt s = if (first_is_minus s) then 0-t
+End
+
+        
+EVAL“LENGTH "1234"”;
+EVAL“SUBSTRING ("1234", 0, 4)”  ;
+EVAL“ -1:int * (toNum "4"):int ”;
+
+
+toNum parsed_digits_string
+        
+
+type_of“minus_parser.run”;
+EVAL “minus_parser.run (Input 0 "-123")”;
+type_of“minus_parser.run”;
+EVAL“first_is_digit "1"”;
+
+EVAL“(0-2):int”;
+type_of“(0-2):int”;
+type_of“(3:num):int”;
+
+(* ----- *)
+
+
+
+(*
+  This module contains a datatype for representing JSON objects, and
+  related functions. A JSON object can be an array of objects, a
+  string, an int, a bool or null, or it can be an object enclosed
+  in {}, in which case it can be viewed as a key-value store of names
+  (strings) and JSON objects.
+*)
+open preamble mlintTheory mlstringTheory
 
 val _ = new_theory"jsonLang";
 
@@ -969,27 +2418,30 @@ val encode_str_def = Define`
 
 Definition json_to_mlstring_def:
   (json_to_mlstring obj = 
-    case obj of
-        | Object mems => List [strlit "{"] ++
-                concat_with (MAP mem_to_string mems) (List [strlit ","]) ++
-                List [strlit "}"]
-        | Array obs => List [strlit "["] ++
-                concat_with (MAP json_to_mlstring obs) (List [strlit ","]) ++
-                List [strlit "]"]
-       | String s => List ([strlit "\""; encode_str T s; strlit "\""])
-       | Int i => List [toString i]
-       | Bool b => if b then List [strlit "true"] else List [strlit "false"]
-       | Null => List [strlit "null"])
+   case obj of
+   | Object mems => List [strlit "{"] ++
+                    concat_with (MAP mem_to_string mems) (List [strlit ","]) ++
+                    List [strlit "}"]
+   | Array obs => List [strlit "["] ++
+                  concat_with (MAP json_to_mlstring obs) (List [strlit ","]) ++
+                  List [strlit "]"]
+   | String s => List ([strlit "\""; encode_str T s; strlit "\""])
+   | Int i => List [toString i]
+   | Bool b => if b then List [strlit "true"] else List [strlit "false"]
+   | Null => List [strlit "null"])
   /\
   (mem_to_string n_obj = let (n, obj) = n_obj in
-        List [strlit "\""; n; strlit "\":"] ++ json_to_mlstring obj)
+                           List [strlit "\""; n; strlit "\":"] ++ json_to_mlstring obj)
+End
 Termination
-   WF_REL_TAC `measure (\x. case x of
-       | INL obj => obj_size obj
-       | INR p => obj2_size p)` \\ rw []
+  WF_REL_TAC `measure (\x. case x of
+                           | INL obj => obj_size obj
+                           | INR p => obj2_size p)` >>
+  rw []>>
 End
 
 val _ = export_theory();
-
-
+type_of“obj_size (Array [])”;
+EVAL“obj_size (Array [Int 1; Int 2; Int 3])”;
+type_of“obj2_size”;
 
